pulse/pulse2rust/src/Pulse2Rust.Rust.Syntax.fst
@@ -44,6 +44,9 @@ let mk_named_typ (s:string) (generic_args:list typ) : typ =
     { typ_path_segment_name = s; typ_path_segment_generic_args = generic_args };
   ]
 
+let mk_fn_typ (typ_fn_args:list typ) (typ_fn_ret:typ) : typ =
+  Typ_fn { typ_fn_args; typ_fn_ret }
+
 let mk_expr_path_singl s = Expr_path [s]
 let mk_expr_path l = Expr_path l
 
