pulse/share/steel/examples/pulse/lib/Pulse.Lib.HashTable.fst
@@ -15,6 +15,7 @@ type pos_us = n:SZ.t{SZ.v n > 0}
 
 let mk_used_cell (#a:eqtype) #b (k:a) (v:b) : cell a b = Used k v
 
+[@@ no_auto_projectors]
 noeq
 type ht_t (keyt:eqtype) (valt:Type) = {
   sz : pos_us;
@@ -29,7 +30,7 @@ let mk_ht (#k:eqtype) #v
   : ht_t k v
   = { sz; hashf; contents; }
 
-let lift_hash_fun (#k:eqtype) (hashf:k -> SZ.t) : k -> nat = fun k -> SZ.v (hashf k)
+let lift_hash_fun (#k:eqtype) (hashf:k -> SZ.t) : GTot (k -> nat) = fun k -> SZ.v (hashf k)
 
 let mk_init_pht (#k:eqtype) #v (hashf:k -> SZ.t) (sz:pos_us)
   : GTot (pht_t k v)
@@ -42,27 +43,21 @@ let mk_init_pht (#k:eqtype) #v (hashf:k -> SZ.t) (sz:pos_us)
     };
     inv = (); }
 
-let related #kt #vt (ht:ht_t kt vt) (pht:pht_t kt vt) : prop =
-    SZ.v ht.sz == pht.repr.sz /\
-    pht.repr.hashf == lift_hash_fun ht.hashf
+let related #kt #vt (ht:ht_t kt vt) (pht:pht_t kt vt) : GTot prop =
+  SZ.v ht.sz == pht.repr.sz /\
+  pht.repr.hashf == lift_hash_fun ht.hashf
 
-let models #kt #vt (ht:ht_t kt vt) (pht:pht_t kt vt) : vprop
-= V.pts_to ht.contents pht.repr.seq **
-  pure (
-    related ht pht /\
-    V.is_full_vec ht.contents
-  )
+let models #kt #vt (ht:ht_t kt vt) (pht:pht_t kt vt) : vprop =
+  V.pts_to ht.contents pht.repr.seq **
+  pure ( related ht pht /\ V.is_full_vec ht.contents)
 
 let pht_sz #k #v (pht:pht_t k v) : GTot pos = pht.repr.sz
 
+noextract
 type exploded_refs (k:eqtype) (v:Type0) =
   ref pos_us &
   ref (k -> SZ.t) &
   ref (V.vec (cell k v))
-
-let tfst (x:'a & 'b & 'c) : 'a = Mktuple3?._1 x
-let tsnd (x:'a & 'b & 'c) : 'b = Mktuple3?._2 x
-let tthd (x:'a & 'b & 'c) : 'c = Mktuple3?._3 x
 
 let token (#k:eqtype) (#v:Type0) (r:ref (ht_t k v)) (res:exploded_refs k v) : vprop =
   exists* ht. pts_to r ht
@@ -133,7 +128,6 @@ fn dealloc (#k:eqtype) (#v:Type0) (ht:ht_t k v)
   ensures emp
 {
   open SZ;
-  let mut off = 0sz;
   with pht. assert (models ht pht);
   unfold (models ht pht);
   V.free ht.contents;
@@ -153,31 +147,8 @@ let sz_add (x y : SZ.t)
 
 
 let size_t_mod (x:SZ.t) (y : SZ.t { y =!= 0sz }) 
-  : z:SZ.t { SZ.v z == SZ.v x % SZ.v y }
+: z:SZ.t { SZ.v z == SZ.v x % SZ.v y }
   = SZ.(x %^ y)
-
-assume val ref_apply (#a #b:Type) (#f:erased (a -> b)) (r:ref (a -> b)) (x:a)
-  : stt b
-    (requires pts_to r f)
-    (ensures fun y -> pts_to r f ** pure (y == (reveal f) x))
-
-assume val vec_ref_read (#a:Type0) (r:ref (V.vec a))
-  (i:SZ.t)
-  (#v:erased (V.vec a))
-  (#s:erased (Seq.seq a) { SZ.v i < Seq.length s})
-  : stt a
-    (requires pts_to r v ** V.pts_to v s)
-    (ensures fun res -> pts_to r v ** V.pts_to v s ** pure (res == Seq.index s (SZ.v i)))
-
-assume val vec_ref_write (#a:Type0) (r:ref (V.vec a))
-  (i:SZ.t)
-  (x:a)
-  (#v:erased (V.vec a))
-  (#s:erased (Seq.seq a) { SZ.v i < Seq.length s})
-  : stt unit
-    (requires pts_to r v ** V.pts_to v s)
-    (ensures fun _ -> pts_to r v ** V.pts_to v (Seq.upd s (SZ.v i) x))
-
 
 #push-options "--z3rlimit_factor 4 --query_stats"
 ```pulse
@@ -185,7 +156,7 @@ fn pulse_lookup_index (#kt:eqtype) (#vt:Type0)
   (#ht:erased (ht_t kt vt))
   (#pht:erased (pht_t kt vt))
   (r:ref (ht_t kt vt))
-  (res:exploded_refs kt vt)
+  (res:(ref pos_us & ref (kt -> SZ.t) & ref (V.vec (cell kt vt))))
   (k:kt)
   requires exploded_vp r ht res ** models ht pht
   returns  p:bool & option (vt & SZ.t)
@@ -243,7 +214,7 @@ fn pulse_lookup_index (#kt:eqtype) (#vt:Type0)
           let idx = size_t_mod sum sz;
           rewrite (V.pts_to ht.contents pht.repr.seq)
                as (V.pts_to (reveal (hide ht.contents)) (reveal (hide pht.repr.seq)));
-          let c = vec_ref_read (tthd res) idx;
+          let c = V.vec_ref_read (tthd res) idx;
           rewrite (V.pts_to (reveal (hide ht.contents)) (reveal (hide pht.repr.seq)))
                as (V.pts_to ht.contents pht.repr.seq);
           match c
@@ -307,441 +278,441 @@ fn pulse_lookup_index (#kt:eqtype) (#vt:Type0)
 #pop-options
 
 
-```pulse
-fn lookup (#kt:eqtype) (#vt:Type0)
-  (r:ref (ht_t kt vt)) (k:kt)
-  (#ht:erased (ht_t kt vt))
-  (#pht:erased (pht_t kt vt))
-  requires pts_to r ht ** models ht pht
-  returns  p:bool & option vt
-  ensures  pts_to r ht ** models ht pht ** 
-           pure ( fst p ==> (snd p) == PHT.lookup pht k )
-{
-  let res = explode_ref r;
-  let p = pulse_lookup_index r res k;
-  unexplode_ref r res;
-  if (fst p)
-  {
-    match (snd p)
-    {
-      Some p -> { (true, Some (fst p)) }
-      None -> { (true, None #vt) }
-    }
-  } 
-  else
-  {
-    (false, None #vt)
-  }
-}
-```
+// ```pulse
+// fn lookup (#kt:eqtype) (#vt:Type0)
+//   (r:ref (ht_t kt vt)) (k:kt)
+//   (#ht:erased (ht_t kt vt))
+//   (#pht:erased (pht_t kt vt))
+//   requires pts_to r ht ** models ht pht
+//   returns  p:bool & option vt
+//   ensures  pts_to r ht ** models ht pht ** 
+//            pure ( fst p ==> (snd p) == PHT.lookup pht k )
+// {
+//   let res = explode_ref r;
+//   let p = pulse_lookup_index r res k;
+//   unexplode_ref r res;
+//   if (fst p)
+//   {
+//     match (snd p)
+//     {
+//       Some p -> { (true, Some (fst p)) }
+//       None -> { (true, None #vt) }
+//     }
+//   } 
+//   else
+//   {
+//     (false, None #vt)
+//   }
+// }
+// ```
 
-```pulse
-fn insert (#kt:eqtype) (#vt:Type0)
-  (r:ref (ht_t kt vt)) (k:kt) (v:vt)
-  (#ht:erased (ht_t kt vt))
-  (#pht:(p:erased (pht_t kt vt) { PHT.not_full p.repr }))
+// ```pulse
+// fn insert (#kt:eqtype) (#vt:Type0)
+//   (r:ref (ht_t kt vt)) (k:kt) (v:vt)
+//   (#ht:erased (ht_t kt vt))
+//   (#pht:(p:erased (pht_t kt vt) { PHT.not_full p.repr }))
   
-  requires pts_to r ht ** models ht pht
-  returns b:bool
-  ensures exists pht'.
-    pts_to r ht ** models ht pht' **
-    pure (if b
-          then pht'== PHT.insert pht k v
-          else pht'== pht)
-{
-  let res = explode_ref r;
+//   requires pts_to r ht ** models ht pht
+//   returns b:bool
+//   ensures exists pht'.
+//     pts_to r ht ** models ht pht' **
+//     pure (if b
+//           then pht'== PHT.insert pht k v
+//           else pht'== pht)
+// {
+//   let res = explode_ref r;
 
-  unfold (exploded_vp r ht res);
-  let sz = !(tfst res);
-  let hash = ref_apply (tsnd res) k;
-  fold (exploded_vp r ht res);
+//   unfold (exploded_vp r ht res);
+//   let sz = !(tfst res);
+//   let hash = ref_apply (tsnd res) k;
+//   fold (exploded_vp r ht res);
 
-  let cidx = size_t_mod hash sz;
-  let mut off = 0sz;
-  let mut cont = true;
-  let mut err = false;
+//   let cidx = size_t_mod hash sz;
+//   let mut off = 0sz;
+//   let mut cont = true;
+//   let mut err = false;
 
-  unfold (models ht pht);
-  while
-  (
-    let vcont = !cont;
-    let verr = !err;
-    (vcont = true && verr = false)
-  ) 
-  invariant b. exists (voff:SZ.t) (vcont verr:bool). (
-    exploded_vp r ht res **
-    R.pts_to off voff **
-    R.pts_to cont vcont **
-    R.pts_to err verr **
-    V.pts_to ht.contents (if (vcont || verr) then pht.repr.seq else (PHT.insert pht k v).repr.seq) **
-    pure (
-      related ht pht /\
-      SZ.(voff <=^ ht.sz) /\
-      strong_all_used_not_by pht.repr (SZ.v cidx) (SZ.v voff) k /\
-      walk pht.repr (SZ.v cidx) k (SZ.v voff) == lookup_repr pht.repr k /\
-      insert_repr_walk #kt #vt #(pht_sz pht) #pht.spec pht.repr k v (SZ.v voff) (SZ.v cidx) () () 
-        == insert_repr #kt #vt #(pht_sz pht) #pht.spec pht.repr k v /\
-      b == (vcont = true && verr = false)
-    ))
-  {
-    unfold (exploded_vp r ht res);
-    let voff = !off;
-    if (voff = sz)
-    {
-      cont := false;
-      full_not_full pht.repr k;
-      assert (V.pts_to ht.contents pht.repr.seq);
-      fold (exploded_vp r ht res);
-    }
-    else
-    {
-      let opt_sum = cidx `sz_add` voff;
-      match opt_sum
-      {
-        Some sum ->
-        {
-          let idx = size_t_mod sum sz;
-          rewrite (V.pts_to ht.contents pht.repr.seq)
-               as (V.pts_to (reveal (hide ht.contents)) (reveal (hide pht.repr.seq)));
-          let c = vec_ref_read (tthd res) idx;
-          rewrite (V.pts_to (reveal (hide ht.contents)) (reveal (hide pht.repr.seq)))
-               as (V.pts_to ht.contents pht.repr.seq);
+//   unfold (models ht pht);
+//   while
+//   (
+//     let vcont = !cont;
+//     let verr = !err;
+//     (vcont = true && verr = false)
+//   ) 
+//   invariant b. exists (voff:SZ.t) (vcont verr:bool). (
+//     exploded_vp r ht res **
+//     R.pts_to off voff **
+//     R.pts_to cont vcont **
+//     R.pts_to err verr **
+//     V.pts_to ht.contents (if (vcont || verr) then pht.repr.seq else (PHT.insert pht k v).repr.seq) **
+//     pure (
+//       related ht pht /\
+//       SZ.(voff <=^ ht.sz) /\
+//       strong_all_used_not_by pht.repr (SZ.v cidx) (SZ.v voff) k /\
+//       walk pht.repr (SZ.v cidx) k (SZ.v voff) == lookup_repr pht.repr k /\
+//       insert_repr_walk #kt #vt #(pht_sz pht) #pht.spec pht.repr k v (SZ.v voff) (SZ.v cidx) () () 
+//         == insert_repr #kt #vt #(pht_sz pht) #pht.spec pht.repr k v /\
+//       b == (vcont = true && verr = false)
+//     ))
+//   {
+//     unfold (exploded_vp r ht res);
+//     let voff = !off;
+//     if (voff = sz)
+//     {
+//       cont := false;
+//       full_not_full pht.repr k;
+//       assert (V.pts_to ht.contents pht.repr.seq);
+//       fold (exploded_vp r ht res);
+//     }
+//     else
+//     {
+//       let opt_sum = cidx `sz_add` voff;
+//       match opt_sum
+//       {
+//         Some sum ->
+//         {
+//           let idx = size_t_mod sum sz;
+//           rewrite (V.pts_to ht.contents pht.repr.seq)
+//                as (V.pts_to (reveal (hide ht.contents)) (reveal (hide pht.repr.seq)));
+//           let c = vec_ref_read (tthd res) idx;
+//           rewrite (V.pts_to (reveal (hide ht.contents)) (reveal (hide pht.repr.seq)))
+//                as (V.pts_to ht.contents pht.repr.seq);
 
-          match c
-          {
-            Used k' v' -> { 
-              if (k' = k) {
-                assert (V.pts_to ht.contents pht.repr.seq);
-                assert (pure ( SZ.v idx < Seq.length pht.repr.seq));
-                rewrite (V.pts_to ht.contents pht.repr.seq)
-                     as (V.pts_to (reveal (hide ht.contents)) (reveal (hide pht.repr.seq)));
-                vec_ref_write (tthd res) idx (mk_used_cell k v);
-                assert (pure ((insert_repr #kt #vt #(pht_sz pht) #pht.spec pht.repr k v).seq `Seq.equal` 
-                              Seq.upd pht.repr.seq (SZ.v idx) (mk_used_cell k v)));
-                rewrite (V.pts_to (reveal (hide ht.contents)) (Seq.upd (reveal (hide pht.repr.seq)) (SZ.v idx) (mk_used_cell k v)))
-                     as (V.pts_to ht.contents (insert_repr #kt #vt #(pht_sz pht) #pht.spec pht.repr k v).seq);
-                cont := false;
-                fold (exploded_vp r ht res);
-              } else {
-                off := SZ.(voff +^ 1sz);
-                fold (exploded_vp r ht res);
-              } 
-            }
-            Clean -> {
-              rewrite (V.pts_to ht.contents pht.repr.seq)
-                   as (V.pts_to (reveal (hide ht.contents)) (reveal (hide pht.repr.seq)));
-              vec_ref_write (tthd res) idx (mk_used_cell k v);
-              assert (pure ((insert_repr #kt #vt #(pht_sz pht) #pht.spec pht.repr k v).seq `Seq.equal` 
-                            Seq.upd pht.repr.seq (SZ.v idx) (mk_used_cell k v)));
-              rewrite (V.pts_to (reveal (hide ht.contents)) (Seq.upd (reveal (hide pht.repr.seq)) (SZ.v idx) (mk_used_cell k v)))
-                   as (V.pts_to ht.contents (insert_repr #kt #vt #(pht_sz pht) #pht.spec pht.repr k v).seq);
-              cont := false;
-              fold (exploded_vp r ht res);
-            }
-            Zombie ->
-            {
-              fold (models ht pht);
-              fold (exploded_vp r ht res);
-              let lookup_res = pulse_lookup_index r res k;
-              unfold (models ht pht);
-              unfold (exploded_vp r ht res);
+//           match c
+//           {
+//             Used k' v' -> { 
+//               if (k' = k) {
+//                 assert (V.pts_to ht.contents pht.repr.seq);
+//                 assert (pure ( SZ.v idx < Seq.length pht.repr.seq));
+//                 rewrite (V.pts_to ht.contents pht.repr.seq)
+//                      as (V.pts_to (reveal (hide ht.contents)) (reveal (hide pht.repr.seq)));
+//                 vec_ref_write (tthd res) idx (mk_used_cell k v);
+//                 assert (pure ((insert_repr #kt #vt #(pht_sz pht) #pht.spec pht.repr k v).seq `Seq.equal` 
+//                               Seq.upd pht.repr.seq (SZ.v idx) (mk_used_cell k v)));
+//                 rewrite (V.pts_to (reveal (hide ht.contents)) (Seq.upd (reveal (hide pht.repr.seq)) (SZ.v idx) (mk_used_cell k v)))
+//                      as (V.pts_to ht.contents (insert_repr #kt #vt #(pht_sz pht) #pht.spec pht.repr k v).seq);
+//                 cont := false;
+//                 fold (exploded_vp r ht res);
+//               } else {
+//                 off := SZ.(voff +^ 1sz);
+//                 fold (exploded_vp r ht res);
+//               } 
+//             }
+//             Clean -> {
+//               rewrite (V.pts_to ht.contents pht.repr.seq)
+//                    as (V.pts_to (reveal (hide ht.contents)) (reveal (hide pht.repr.seq)));
+//               vec_ref_write (tthd res) idx (mk_used_cell k v);
+//               assert (pure ((insert_repr #kt #vt #(pht_sz pht) #pht.spec pht.repr k v).seq `Seq.equal` 
+//                             Seq.upd pht.repr.seq (SZ.v idx) (mk_used_cell k v)));
+//               rewrite (V.pts_to (reveal (hide ht.contents)) (Seq.upd (reveal (hide pht.repr.seq)) (SZ.v idx) (mk_used_cell k v)))
+//                    as (V.pts_to ht.contents (insert_repr #kt #vt #(pht_sz pht) #pht.spec pht.repr k v).seq);
+//               cont := false;
+//               fold (exploded_vp r ht res);
+//             }
+//             Zombie ->
+//             {
+//               fold (models ht pht);
+//               fold (exploded_vp r ht res);
+//               let lookup_res = pulse_lookup_index r res k;
+//               unfold (models ht pht);
+//               unfold (exploded_vp r ht res);
 
-              if (fst lookup_res)
-              {
-                let o = snd lookup_res;
-                match o
-                {
-                  Some p ->
-                  {
-                    rewrite (V.pts_to ht.contents pht.repr.seq)
-                         as (V.pts_to (reveal (hide ht.contents)) (reveal (hide pht.repr.seq)));
-                    vec_ref_write (tthd res) (snd p) Zombie;
-                    vec_ref_write (tthd res) idx (mk_used_cell k v);
-                    cont := false;
-                    assert (pure ((insert_repr #kt #vt #(pht_sz pht) #pht.spec pht.repr k v).seq `Seq.equal` 
-                                  Seq.upd (Seq.upd pht.repr.seq (SZ.v (snd p)) Zombie) (SZ.v idx) (mk_used_cell k v)));
-                    rewrite (V.pts_to (reveal (hide ht.contents))
-                                      (Seq.upd (Seq.upd (reveal (hide pht.repr.seq)) (SZ.v (snd p)) Zombie) (SZ.v idx) (mk_used_cell k v)))
-                         as (V.pts_to ht.contents (insert_repr #kt #vt #(pht_sz pht) #pht.spec pht.repr k v).seq);
-                    fold (exploded_vp r ht res);
-                  }
-                  None ->
-                  {
-                    rewrite (V.pts_to ht.contents pht.repr.seq)
-                         as (V.pts_to (reveal (hide ht.contents)) (reveal (hide pht.repr.seq)));
-                    vec_ref_write (tthd res) idx (mk_used_cell k v);                    
-                    cont := false;
-                    assert (pure ((insert_repr #kt #vt #(pht_sz pht) #pht.spec pht.repr k v).seq `Seq.equal`
-                                  Seq.upd pht.repr.seq (SZ.v idx) (mk_used_cell k v)));
-                    rewrite (V.pts_to (reveal (hide ht.contents)) (Seq.upd (reveal (hide pht.repr.seq)) (SZ.v idx) (mk_used_cell k v)))
-                         as (V.pts_to ht.contents (insert_repr #kt #vt #(pht_sz pht) #pht.spec pht.repr k v).seq);
-                    fold (exploded_vp r ht res);
-                  }
-                }
-              }
-              else
-              {
-                // ERROR - lookup failed
-                err := true;
-                fold (exploded_vp r ht res);
-              }
-            }
-          }
-        }
-        None ->
-        {
-          // ERROR - add failed
-          err := true;
-          fold (exploded_vp r ht res);
-        }
-      }
-    }
-  };
-  unexplode_ref r res;
-  let verr = !err;
-  if verr
-  {
-    fold (models ht pht);
-    false
-  } else {
-    assert (V.pts_to ht.contents (PHT.insert pht k v).repr.seq);
-    fold (models ht (PHT.insert pht k v));
-    true
-  }
-}
-```
+//               if (fst lookup_res)
+//               {
+//                 let o = snd lookup_res;
+//                 match o
+//                 {
+//                   Some p ->
+//                   {
+//                     rewrite (V.pts_to ht.contents pht.repr.seq)
+//                          as (V.pts_to (reveal (hide ht.contents)) (reveal (hide pht.repr.seq)));
+//                     vec_ref_write (tthd res) (snd p) Zombie;
+//                     vec_ref_write (tthd res) idx (mk_used_cell k v);
+//                     cont := false;
+//                     assert (pure ((insert_repr #kt #vt #(pht_sz pht) #pht.spec pht.repr k v).seq `Seq.equal` 
+//                                   Seq.upd (Seq.upd pht.repr.seq (SZ.v (snd p)) Zombie) (SZ.v idx) (mk_used_cell k v)));
+//                     rewrite (V.pts_to (reveal (hide ht.contents))
+//                                       (Seq.upd (Seq.upd (reveal (hide pht.repr.seq)) (SZ.v (snd p)) Zombie) (SZ.v idx) (mk_used_cell k v)))
+//                          as (V.pts_to ht.contents (insert_repr #kt #vt #(pht_sz pht) #pht.spec pht.repr k v).seq);
+//                     fold (exploded_vp r ht res);
+//                   }
+//                   None ->
+//                   {
+//                     rewrite (V.pts_to ht.contents pht.repr.seq)
+//                          as (V.pts_to (reveal (hide ht.contents)) (reveal (hide pht.repr.seq)));
+//                     vec_ref_write (tthd res) idx (mk_used_cell k v);                    
+//                     cont := false;
+//                     assert (pure ((insert_repr #kt #vt #(pht_sz pht) #pht.spec pht.repr k v).seq `Seq.equal`
+//                                   Seq.upd pht.repr.seq (SZ.v idx) (mk_used_cell k v)));
+//                     rewrite (V.pts_to (reveal (hide ht.contents)) (Seq.upd (reveal (hide pht.repr.seq)) (SZ.v idx) (mk_used_cell k v)))
+//                          as (V.pts_to ht.contents (insert_repr #kt #vt #(pht_sz pht) #pht.spec pht.repr k v).seq);
+//                     fold (exploded_vp r ht res);
+//                   }
+//                 }
+//               }
+//               else
+//               {
+//                 // ERROR - lookup failed
+//                 err := true;
+//                 fold (exploded_vp r ht res);
+//               }
+//             }
+//           }
+//         }
+//         None ->
+//         {
+//           // ERROR - add failed
+//           err := true;
+//           fold (exploded_vp r ht res);
+//         }
+//       }
+//     }
+//   };
+//   unexplode_ref r res;
+//   let verr = !err;
+//   if verr
+//   {
+//     fold (models ht pht);
+//     false
+//   } else {
+//     assert (V.pts_to ht.contents (PHT.insert pht k v).repr.seq);
+//     fold (models ht (PHT.insert pht k v));
+//     true
+//   }
+// }
+// ```
 
-```pulse
-fn delete (#kt:eqtype) (#vt:Type0)
-  (r:ref (ht_t kt vt)) (k:kt)
-  (#ht:erased (ht_t kt vt))
-  (#pht:erased (pht_t kt vt))
-  requires pts_to r ht ** models ht pht
-  returns b:bool
-  ensures exists pht'.
-    pts_to r ht **
-    models ht pht' **
-    pure (if b then pht' == PHT.delete pht k else pht' == pht)
-{
-  let res = explode_ref r;
+// ```pulse
+// fn delete (#kt:eqtype) (#vt:Type0)
+//   (r:ref (ht_t kt vt)) (k:kt)
+//   (#ht:erased (ht_t kt vt))
+//   (#pht:erased (pht_t kt vt))
+//   requires pts_to r ht ** models ht pht
+//   returns b:bool
+//   ensures exists pht'.
+//     pts_to r ht **
+//     models ht pht' **
+//     pure (if b then pht' == PHT.delete pht k else pht' == pht)
+// {
+//   let res = explode_ref r;
 
-  unfold (exploded_vp r ht res);
-  let sz = !(tfst res);
-  let hash = ref_apply (tsnd res) k;
-  fold (exploded_vp r ht res);
+//   unfold (exploded_vp r ht res);
+//   let sz = !(tfst res);
+//   let hash = ref_apply (tsnd res) k;
+//   fold (exploded_vp r ht res);
 
-  let cidx = size_t_mod hash sz;
-  let mut off = 0sz;
-  let mut cont = true;
-  let mut err = false;
+//   let cidx = size_t_mod hash sz;
+//   let mut off = 0sz;
+//   let mut cont = true;
+//   let mut err = false;
 
-  unfold (models ht pht);
-  while 
-  (
-    let vcont = !cont;
-    let verr = !err; 
-    (vcont = true && verr = false)
-  )
-  invariant b. exists (voff:SZ.t) (vcont verr:bool). (
-    exploded_vp r ht res **
-    R.pts_to off voff **
-    R.pts_to cont vcont **
-    R.pts_to err verr **
-    V.pts_to ht.contents (if (vcont || verr) then pht.repr.seq else (PHT.delete pht k).repr.seq) **
-    pure (
-      SZ.v ht.sz == pht_sz pht /\
-      SZ.(voff <=^ ht.sz) /\
-      all_used_not_by pht.repr (SZ.v cidx) (SZ.v voff) k /\
-      walk pht.repr (SZ.v cidx) k (SZ.v voff) == lookup_repr pht.repr k /\
-      delete_repr_walk #kt #vt #(pht_sz pht) #pht.spec pht.repr k (SZ.v voff) (SZ.v cidx) () () 
-        == delete_repr #kt #vt #(pht_sz pht) #pht.spec pht.repr k /\
-      b == (vcont = true && verr = false)
-    ))
-  {
-    unfold (exploded_vp r ht res);
-    let voff = !off;
-    if (voff = sz)
-    {
-      cont := false;
-      assert (V.pts_to ht.contents pht.repr.seq);
-      fold (exploded_vp r ht res);
-    }
-    else
-    {
-      let opt_sum = cidx `sz_add` voff;
-      match opt_sum
-      {
-        Some sum ->
-        {
-          let idx = size_t_mod sum sz;
-          rewrite (V.pts_to ht.contents pht.repr.seq)
-               as (V.pts_to (reveal (hide ht.contents)) (reveal (hide pht.repr.seq)));
-          let c = vec_ref_read (tthd res) idx;
-          rewrite (V.pts_to (reveal (hide ht.contents)) (reveal (hide pht.repr.seq)))
-               as (V.pts_to ht.contents pht.repr.seq);
+//   unfold (models ht pht);
+//   while 
+//   (
+//     let vcont = !cont;
+//     let verr = !err; 
+//     (vcont = true && verr = false)
+//   )
+//   invariant b. exists (voff:SZ.t) (vcont verr:bool). (
+//     exploded_vp r ht res **
+//     R.pts_to off voff **
+//     R.pts_to cont vcont **
+//     R.pts_to err verr **
+//     V.pts_to ht.contents (if (vcont || verr) then pht.repr.seq else (PHT.delete pht k).repr.seq) **
+//     pure (
+//       SZ.v ht.sz == pht_sz pht /\
+//       SZ.(voff <=^ ht.sz) /\
+//       all_used_not_by pht.repr (SZ.v cidx) (SZ.v voff) k /\
+//       walk pht.repr (SZ.v cidx) k (SZ.v voff) == lookup_repr pht.repr k /\
+//       delete_repr_walk #kt #vt #(pht_sz pht) #pht.spec pht.repr k (SZ.v voff) (SZ.v cidx) () () 
+//         == delete_repr #kt #vt #(pht_sz pht) #pht.spec pht.repr k /\
+//       b == (vcont = true && verr = false)
+//     ))
+//   {
+//     unfold (exploded_vp r ht res);
+//     let voff = !off;
+//     if (voff = sz)
+//     {
+//       cont := false;
+//       assert (V.pts_to ht.contents pht.repr.seq);
+//       fold (exploded_vp r ht res);
+//     }
+//     else
+//     {
+//       let opt_sum = cidx `sz_add` voff;
+//       match opt_sum
+//       {
+//         Some sum ->
+//         {
+//           let idx = size_t_mod sum sz;
+//           rewrite (V.pts_to ht.contents pht.repr.seq)
+//                as (V.pts_to (reveal (hide ht.contents)) (reveal (hide pht.repr.seq)));
+//           let c = vec_ref_read (tthd res) idx;
+//           rewrite (V.pts_to (reveal (hide ht.contents)) (reveal (hide pht.repr.seq)))
+//                as (V.pts_to ht.contents pht.repr.seq);
 
-          match c
-          {
-            Used k' v' ->
-            { 
-              if (k' = k)
-              {
-                rewrite (V.pts_to ht.contents pht.repr.seq)
-                     as (V.pts_to (reveal (hide ht.contents)) (reveal (hide pht.repr.seq)));
-                vec_ref_write (tthd res) idx Zombie;
-                cont := false;
-                assert (pure (pht.repr @@ SZ.v idx == Used k v'));
-                assert (pure (Seq.upd pht.repr.seq (SZ.v idx) Zombie  `Seq.equal`
-                              (PHT.delete pht k).repr.seq));
-                rewrite (V.pts_to (reveal (hide ht.contents)) (Seq.upd (reveal (hide pht.repr.seq)) (SZ.v idx) Zombie))
-                     as (V.pts_to ht.contents (PHT.delete pht k).repr.seq);
-                fold (exploded_vp r ht res);
-              }
-              else
-              {
-                off := SZ.(voff +^ 1sz);
-                fold (exploded_vp r ht res);
-              } 
-            }
-            Clean ->
-            {
-              cont := false;
-              assert (pure (pht.repr == (PHT.delete pht k).repr));
-              fold (exploded_vp r ht res);
-            }
-            Zombie ->
-            {
-              off := SZ.(voff +^ 1sz);
-              fold (exploded_vp r ht res);
-            }
-          }
-        }
-        None ->
-        {
-          // ERROR - add failed
-          err := false;
-          fold (exploded_vp r ht res);
-        }
-      }
-    }
-  };
-  unexplode_ref r res;
-  let verr = !err;
-  if verr
-  {
-    fold (models ht pht);
-    false
-  }
-  else
-  {
-    fold (models ht (PHT.delete pht k));
-    true
-  }
-}
-```
+//           match c
+//           {
+//             Used k' v' ->
+//             { 
+//               if (k' = k)
+//               {
+//                 rewrite (V.pts_to ht.contents pht.repr.seq)
+//                      as (V.pts_to (reveal (hide ht.contents)) (reveal (hide pht.repr.seq)));
+//                 vec_ref_write (tthd res) idx Zombie;
+//                 cont := false;
+//                 assert (pure (pht.repr @@ SZ.v idx == Used k v'));
+//                 assert (pure (Seq.upd pht.repr.seq (SZ.v idx) Zombie  `Seq.equal`
+//                               (PHT.delete pht k).repr.seq));
+//                 rewrite (V.pts_to (reveal (hide ht.contents)) (Seq.upd (reveal (hide pht.repr.seq)) (SZ.v idx) Zombie))
+//                      as (V.pts_to ht.contents (PHT.delete pht k).repr.seq);
+//                 fold (exploded_vp r ht res);
+//               }
+//               else
+//               {
+//                 off := SZ.(voff +^ 1sz);
+//                 fold (exploded_vp r ht res);
+//               } 
+//             }
+//             Clean ->
+//             {
+//               cont := false;
+//               assert (pure (pht.repr == (PHT.delete pht k).repr));
+//               fold (exploded_vp r ht res);
+//             }
+//             Zombie ->
+//             {
+//               off := SZ.(voff +^ 1sz);
+//               fold (exploded_vp r ht res);
+//             }
+//           }
+//         }
+//         None ->
+//         {
+//           // ERROR - add failed
+//           err := false;
+//           fold (exploded_vp r ht res);
+//         }
+//       }
+//     }
+//   };
+//   unexplode_ref r res;
+//   let verr = !err;
+//   if verr
+//   {
+//     fold (models ht pht);
+//     false
+//   }
+//   else
+//   {
+//     fold (models ht (PHT.delete pht k));
+//     true
+//   }
+// }
+// ```
 
-```pulse
-fn not_full (#kt:eqtype) (#vt:Type0)
-  (r:ref (ht_t kt vt))
-  (#ht:erased (ht_t kt vt))
-  (#pht:erased (pht_t kt vt))
-  requires pts_to r ht ** models ht pht
-  returns b:bool
-  ensures pts_to r ht ** models ht pht ** 
-          pure (b ==> PHT.not_full pht.repr)
-{
-  let res = explode_ref r;
+// ```pulse
+// fn not_full (#kt:eqtype) (#vt:Type0)
+//   (r:ref (ht_t kt vt))
+//   (#ht:erased (ht_t kt vt))
+//   (#pht:erased (pht_t kt vt))
+//   requires pts_to r ht ** models ht pht
+//   returns b:bool
+//   ensures pts_to r ht ** models ht pht ** 
+//           pure (b ==> PHT.not_full pht.repr)
+// {
+//   let res = explode_ref r;
 
-  let mut i = 0sz;
-  unfold (models ht pht);
+//   let mut i = 0sz;
+//   unfold (models ht pht);
 
-  unfold (exploded_vp r ht res);
-  let sz = !(tfst res);
-  fold (exploded_vp r ht res);
+//   unfold (exploded_vp r ht res);
+//   let sz = !(tfst res);
+//   fold (exploded_vp r ht res);
 
-  while
-  (
-    let vi = !i;  
-    if SZ.(vi <^ sz)
-    {
-      unfold (exploded_vp r ht res);
-      rewrite (V.pts_to ht.contents pht.repr.seq)
-           as (V.pts_to (reveal (hide ht.contents)) (reveal (hide pht.repr.seq)));
-      let c = vec_ref_read (tthd res) vi;
-      rewrite (V.pts_to (reveal (hide ht.contents)) (reveal (hide pht.repr.seq)))
-           as (V.pts_to ht.contents pht.repr.seq);
-      fold (exploded_vp r ht res);
-      (Used? c) 
-    }
-    else 
-    { 
-      false
-    }
-  )
-  invariant b. exists (vi:SZ.t). (
-    exploded_vp r ht res **
-    V.pts_to ht.contents pht.repr.seq **
-    R.pts_to i vi **
-    pure (
-      SZ.v ht.sz == pht_sz pht /\
-      SZ.(vi <=^ ht.sz) /\
-      (b == (SZ.(vi <^ ht.sz) && Used? (pht.repr @@ (SZ.v vi)))) /\
-      (forall (i:nat). i < SZ.v vi ==> Used? (pht.repr @@ i))
-    )
-  )
-  {
-    let vi = !i;
-    i := SZ.(vi +^ 1sz);
-  };
-  unexplode_ref r res;
-  let vi = !i;
-  let res = SZ.(vi <^ sz);
-  fold (models ht pht);  
-  res
-}
-```
+//   while
+//   (
+//     let vi = !i;  
+//     if SZ.(vi <^ sz)
+//     {
+//       unfold (exploded_vp r ht res);
+//       rewrite (V.pts_to ht.contents pht.repr.seq)
+//            as (V.pts_to (reveal (hide ht.contents)) (reveal (hide pht.repr.seq)));
+//       let c = vec_ref_read (tthd res) vi;
+//       rewrite (V.pts_to (reveal (hide ht.contents)) (reveal (hide pht.repr.seq)))
+//            as (V.pts_to ht.contents pht.repr.seq);
+//       fold (exploded_vp r ht res);
+//       (Used? c) 
+//     }
+//     else 
+//     { 
+//       false
+//     }
+//   )
+//   invariant b. exists (vi:SZ.t). (
+//     exploded_vp r ht res **
+//     V.pts_to ht.contents pht.repr.seq **
+//     R.pts_to i vi **
+//     pure (
+//       SZ.v ht.sz == pht_sz pht /\
+//       SZ.(vi <=^ ht.sz) /\
+//       (b == (SZ.(vi <^ ht.sz) && Used? (pht.repr @@ (SZ.v vi)))) /\
+//       (forall (i:nat). i < SZ.v vi ==> Used? (pht.repr @@ i))
+//     )
+//   )
+//   {
+//     let vi = !i;
+//     i := SZ.(vi +^ 1sz);
+//   };
+//   unexplode_ref r res;
+//   let vi = !i;
+//   let res = SZ.(vi <^ sz);
+//   fold (models ht pht);  
+//   res
+// }
+// ```
 
-let hash_us (k:SZ.t) : SZ.t = k
+// let hash_us (k:SZ.t) : SZ.t = k
 
-let init_not_full (#kt:eqtype) (#vt:eqtype) (hashf:kt -> SZ.t) (l:pos_us)
-  : Lemma (Pulse.Lib.HashTable.Spec.not_full (mk_init_pht #kt #vt hashf l).repr)
-  = assert (~(Used? ((mk_init_pht #kt #vt hashf l).repr @@ 0)))
+// let init_not_full (#kt:eqtype) (#vt:eqtype) (hashf:kt -> SZ.t) (l:pos_us)
+//   : Lemma (Pulse.Lib.HashTable.Spec.not_full (mk_init_pht #kt #vt hashf l).repr)
+//   = assert (~(Used? ((mk_init_pht #kt #vt hashf l).repr @@ 0)))
 
-```pulse
-fn test_mono ()
-  requires emp
-  ensures emp
-{
-   let htc = alloc #SZ.t #SZ.t hash_us 128sz;
-   with pht. assert (models htc pht);
-   let ht = R.alloc htc;
-   init_not_full #SZ.t #SZ.t hash_us 128sz;
-   rewrite (models htc pht) as (models (reveal (hide htc)) pht);
-   let b = insert ht 0sz 17sz;
-   if (b) {
-     let v = lookup ht 0sz;
-     if (fst v) {
-       assert pure (snd v == Some 17sz);
-       R.free ht;
-       with pht. assert (models (reveal (hide htc)) pht);
-       rewrite (models (reveal (hide htc)) pht) as (models htc pht);
-       dealloc htc
-     }
-     else {
-      R.free ht;
-      with pht. assert (models (reveal (hide htc)) pht);
-      rewrite (models (reveal (hide htc)) pht) as (models htc pht);
-      dealloc htc
-     }
-   }
-   else {
-    let b = delete ht 0sz;
-    let b' = not_full ht;
-    R.free ht;
-    with pht. assert (models (reveal (hide htc)) pht);
-    rewrite (models (reveal (hide htc)) pht) as (models htc pht);
-    dealloc htc
-   } 
-}
-```
-// let test_mono = test_mono'
+// ```pulse
+// fn test_mono ()
+//   requires emp
+//   ensures emp
+// {
+//    let htc = alloc #SZ.t #SZ.t hash_us 128sz;
+//    with pht. assert (models htc pht);
+//    let ht = R.alloc htc;
+//    init_not_full #SZ.t #SZ.t hash_us 128sz;
+//    rewrite (models htc pht) as (models (reveal (hide htc)) pht);
+//    let b = insert ht 0sz 17sz;
+//    if (b) {
+//      let v = lookup ht 0sz;
+//      if (fst v) {
+//        assert pure (snd v == Some 17sz);
+//        R.free ht;
+//        with pht. assert (models (reveal (hide htc)) pht);
+//        rewrite (models (reveal (hide htc)) pht) as (models htc pht);
+//        dealloc htc
+//      }
+//      else {
+//       R.free ht;
+//       with pht. assert (models (reveal (hide htc)) pht);
+//       rewrite (models (reveal (hide htc)) pht) as (models htc pht);
+//       dealloc htc
+//      }
+//    }
+//    else {
+//     let b = delete ht 0sz;
+//     let b' = not_full ht;
+//     R.free ht;
+//     with pht. assert (models (reveal (hide htc)) pht);
+//     rewrite (models (reveal (hide htc)) pht) as (models htc pht);
+//     dealloc htc
+//    } 
+// }
+// ```
+// // let test_mono = test_mono'
