pulse/share/steel/examples/pulse/lib/Pulse.Lib.Vec.fsti
@@ -8,6 +8,7 @@ module SZ = FStar.SizeT
 module Seq = FStar.Seq
 module T = FStar.Tactics.V2
 
+module R = Pulse.Lib.Reference
 module A = Pulse.Lib.Array.Core
 
 val vec ([@@@strictly_positive] a:Type0) : Type u#0
@@ -79,3 +80,20 @@ val to_vec_pts_to (#a:Type0) (v:vec a) (#p:perm) (#s:Seq.seq a)
   : stt_ghost unit emp_inames
       (A.pts_to (vec_to_array v) #p s)
       (fun _ → pts_to v #p s)
+
+val vec_ref_read (#a:Type0) (r:R.ref (vec a))
+  (i:SZ.t)
+  (#v:erased (vec a))
+  (#s:erased (Seq.seq a) { SZ.v i < Seq.length s})
+  : stt a
+    (requires R.pts_to r v ** pts_to v s)
+    (ensures fun res -> R.pts_to r v ** pts_to v s ** pure (res == Seq.index s (SZ.v i)))
+
+val vec_ref_write (#a:Type0) (r:R.ref (vec a))
+  (i:SZ.t)
+  (x:a)
+  (#v:erased (vec a))
+  (#s:erased (Seq.seq a) { SZ.v i < Seq.length s})
+  : stt unit
+    (requires R.pts_to r v ** pts_to v s)
+    (ensures fun _ -> R.pts_to r v ** pts_to v (Seq.upd s (SZ.v i) x))
